kosaraju-lean4/Kosaraju/Dfs2.lean
@@ -4,18 +4,18 @@ import Std.Data.List.Lemmas
 
 open Rank
 
-structure Funnel [DirectedGraph Node Graph] [BEq Node] [LawfulBEq Node]
+structure Funnel [DirectedGraph V Graph] [BEq V] [LawfulBEq V]
                   (graph: Graph)
-                  (roots black_stack grays : List Node)
+                  (roots black_stack grays : List V)
 where
-  stack : List Node
+  stack : List V
   p₁ : wff_color graph stack grays
   p₂ : roots ⊆ stack ++ grays
   monotony: ∃ s', stack = s' ++ black_stack /\ access_from_set graph roots s'
 
-def dfs2 [DirectedGraph Node Graph] [BEq Node] [LawfulBEq Node]
+def dfs2 [DirectedGraph V Graph] [BEq V] [LawfulBEq V]
          (graph: Graph)
-         (roots black_stack grays : List Node)
+         (roots black_stack grays : List V)
          (h₁: roots ⊆ DirectedGraph.all_nodes graph)
          (h₂: grays ⊆ DirectedGraph.all_nodes graph)
          (h₃: wff_color graph black_stack grays)
@@ -70,7 +70,7 @@ def dfs2 [DirectedGraph Node Graph] [BEq Node] [LawfulBEq Node]
                     . rw [simplelist_tl]
                       simp_all
                       tauto
-    let v : List Node := (DirectedGraph.all_nodes graph)
+    let v : List V := (DirectedGraph.all_nodes graph)
     let termination_proof: grays.length < v.length := by
       apply simplelist_size_2
       . tauto
@@ -186,5 +186,5 @@ def dfs2 [DirectedGraph Node Graph] [BEq Node] [LawfulBEq Node]
                                                   subst a
                                                   tauto
     }
-termination_by let v : List Node := DirectedGraph.all_nodes graph
+termination_by let v : List V := DirectedGraph.all_nodes graph
                (v.length - grays.length, roots)
